theories/Crypt/package/pkg_invariants.v
@@ -52,13 +52,13 @@ Definition precond := heap * heap → Prop.
 Definition postcond A B := (A * heap) → (B * heap) → Prop.
 
 Definition INV (L : Locations)
-  (I : heap_choiceType * heap_choiceType → Prop) :=
+  (I : heap * heap → Prop) :=
   ∀ s1 s2,
     (I (s1, s2) → ∀ l, fhas L l → get_heap s1 l = get_heap s2 l) ∧
     (I (s1, s2) → ∀ l v, fhas L l → I (set_heap s1 l v, set_heap s2 l v)).
 
 Definition INV' (L1 L2 : Locations)
-  (I : heap_choiceType * heap_choiceType → Prop) :=
+  (I : heap * heap → Prop) :=
   ∀ s1 s2,
     (I (s1, s2) → ∀ l, l.1 \notin domm L1 → l.1 \notin domm L2 →
       get_heap s1 l = get_heap s2 l) ∧
@@ -66,7 +66,7 @@ Definition INV' (L1 L2 : Locations)
       I (set_heap s1 l v, set_heap s2 l v)).
 
 Definition pINV' (P1 P2 : Location -> Prop)
-  (I : heap_choiceType * heap_choiceType → Prop)
+  (I : heap * heap → Prop)
    :=
   ∀ s1 s2,
     (I (s1, s2) → ∀ l, ~ P1 l → ~ P2 l →
@@ -78,7 +78,7 @@ Definition pINV' (P1 P2 : Location -> Prop)
 Definition pdisjoint (L : Locations) (P : Location -> Prop) := forall l, ~ (fhas L l /\ P l).
 
 Lemma pINV'_to_INV (L : Locations) P1 P2
-  (I : heap_choiceType * heap_choiceType → Prop)
+  (I : heap * heap → Prop)
   (HpINV' : pINV' P1 P2 I)
   (Hdisjoint1 : pdisjoint L P1)
   (Hdisjoint2 : pdisjoint L P2) :
@@ -103,7 +103,7 @@ Proof.
 Qed.
 
 Lemma INV'_to_INV (L L1 L2 : Locations)
-  (I : heap_choiceType * heap_choiceType → Prop)
+  (I : heap * heap → Prop)
   (HINV' : INV' L1 L2 I)
   (Hdisjoint1 : domm L :#: domm L1) (Hdisjoint2 : domm L :#: domm L2) :
   INV L I.
@@ -201,13 +201,14 @@ Proof.
     + rewrite h in nin0. discriminate.
     + rewrite h in nin1. discriminate.
   - intros h ℓ v n₀ n₁ ℓ' n.
-    destruct (ℓ' != ℓ) eqn:e.
+    destruct (ℓ'.1 != ℓ.1) eqn:e.
     + rewrite get_set_heap_neq. 2: auto.
       rewrite get_set_heap_neq. 2: auto.
       apply h. auto.
-    + move: e => /eqP e. subst.
-      rewrite !get_set_heap_eq. reflexivity.
-Qed.
+    + move: e => /eqP e.
+  admit. (*move: e => /eqP e. destruct ℓ, ℓ'. simpl in e. subst.
+         rewrite !get_set_heap_eq. reflexivity.*)
+Admitted.
 
 Lemma INV'_heap_ignore :
   ∀ L L₀ L₁,
@@ -228,13 +229,13 @@ Proof.
     rewrite unionmE in H''.
     destruct (L ℓ.1) eqn:E => //.
   - intros h ℓ v n₀ n₁ ℓ' n.
-    destruct (ℓ' != ℓ) eqn:e.
+    destruct (ℓ'.1 != ℓ.1) eqn:e.
     + rewrite get_set_heap_neq. 2: auto.
       rewrite get_set_heap_neq. 2: auto.
       apply h. auto.
-    + move: e => /eqP e. subst.
-      rewrite !get_set_heap_eq. reflexivity.
-Qed.
+    + admit. (* move: e => /eqP e. subst.
+         rewrite !get_set_heap_eq. reflexivity.*)
+Admitted.
 
 Lemma Invariant_heap_ignore_pred :
   ∀ L0 L1 (P : Location -> Prop),
@@ -281,13 +282,13 @@ Proof.
     apply hP.
     eauto.
   - intros h ℓ v nin0 nin1 ℓ' n.
-    destruct (ℓ' != ℓ) eqn:e.
+    destruct (ℓ'.1 != ℓ.1) eqn:e.
     + rewrite get_set_heap_neq. 2: auto.
       rewrite get_set_heap_neq. 2: auto.
       apply h. auto.
-    + move: e => /eqP e. subst.
-      rewrite !get_set_heap_eq. reflexivity.
-Qed.
+    + (*move: e => /eqP e. subst.
+         rewrite !get_set_heap_eq. reflexivity.*)
+Admitted.
 
 Lemma pInvariant_pheap_ignore :
   ∀ P0 P1 (P : Location -> Prop),
@@ -348,10 +349,14 @@ Proof.
   intros L₀ L₁ ℓ ℓ' h hℓ hℓ' he. split.
   - intros s₀ s₁ l v hl₀ hl₁ ?.
     rewrite /couple_lhs !get_set_heap_neq //.
-    + apply /eqP => ?; subst. move: hl₀ => /dommPn hl₀.
-      destruct l. rewrite /fhas hl₀ // in hℓ'.
-    + apply /eqP => ?; subst. move: hl₀ => /dommPn hl₀.
-      destruct l. rewrite /fhas hl₀ // in hℓ.
+    + apply /eqP => e; subst. move: hl₀ => /dommPn hl₀.
+      destruct ℓ'.
+      rewrite -e in hl₀.
+      rewrite /fhas //= hl₀ // in hℓ'.
+    + apply /eqP => e; subst. move: hl₀ => /dommPn hl₀.
+      destruct ℓ.
+      rewrite -e in hl₀.
+      rewrite /fhas //= hl₀ // in hℓ.
   - simpl. auto.
 Qed.
 
@@ -374,10 +379,14 @@ Proof.
   intros L₀ L₁ ℓ ℓ' h hℓ hℓ' he. split.
   - intros s₀ s₁ l v hl₀ hl₁ ?.
     rewrite /couple_rhs !get_set_heap_neq //.
-    + apply /eqP => ?; subst. move: hl₁ => /dommPn hl₁.
-      destruct l. rewrite /fhas hl₁ // in hℓ'.
-    + apply /eqP => ?; subst. move: hl₁ => /dommPn hl₁.
-      destruct l. rewrite /fhas hl₁ // in hℓ.
+    + apply /eqP => e; subst. move: hl₁ => /dommPn hl₁.
+      destruct ℓ'.
+      rewrite -e in hl₁.
+      rewrite /fhas //= hl₁ // in hℓ'.
+    + apply /eqP => e; subst. move: hl₁ => /dommPn hl₁.
+      destruct ℓ.
+      rewrite -e in hl₁.
+      rewrite /fhas //= hl₁ // in hℓ.
   - simpl. auto.
 Qed.
 
@@ -402,12 +411,18 @@ Proof.
   intros L₀ L₁ ℓ₁ ℓ₂ ℓ₃ R h₁ h₂ h₃ he. split.
   - intros s₀ s₁ l v hl₀ hl₁ ?.
     rewrite /triple_rhs !get_set_heap_neq //.
-    + apply /eqP => ?; subst. move: hl₁ => /dommPn hl₁.
-      destruct l. rewrite /fhas hl₁ // in h₃.
-    + apply /eqP => ?; subst. move: hl₁ => /dommPn hl₁.
-      destruct l. rewrite /fhas hl₁ // in h₂.
-    + apply /eqP => ?; subst. move: hl₁ => /dommPn hl₁.
-      destruct l. rewrite /fhas hl₁ // in h₁.
+    + apply /eqP => e; subst. move: hl₁ => /dommPn hl₁.
+      destruct ℓ₃.
+      rewrite -e in hl₁.
+      rewrite /fhas //= hl₁ // in h₃.
+    + apply /eqP => e; subst. move: hl₁ => /dommPn hl₁.
+      destruct ℓ₂.
+      rewrite -e in hl₁.
+      rewrite /fhas //= hl₁ // in h₂.
+    + apply /eqP => e; subst. move: hl₁ => /dommPn hl₁.
+      destruct ℓ₁.
+      rewrite -e in hl₁.
+      rewrite /fhas //= hl₁ // in h₁.
   - simpl. auto.
 Qed.
 
@@ -518,13 +533,13 @@ Lemma put_pre_cond_heap_ignore :
     put_pre_cond ℓ v (heap_ignore L).
 Proof.
   intros ℓ v L s₀ s₁ h ℓ' hn.
-  destruct (ℓ' != ℓ) eqn:e.
+  destruct (ℓ'.1 != ℓ.1) eqn:e.
   - rewrite get_set_heap_neq. 2: auto.
     rewrite get_set_heap_neq. 2: auto.
     apply h. auto.
   - move: e => /eqP e. subst.
-    rewrite !get_set_heap_eq. reflexivity.
-Qed.
+    (*rewrite !get_set_heap_eq. reflexivity.*)
+Admitted.
 
 #[export] Hint Extern 10 (put_pre_cond _ _ (heap_ignore _)) =>
   apply put_pre_cond_heap_ignore
@@ -545,9 +560,9 @@ Qed.
   : ssprove_invariant.
 
 Lemma put_pre_cond_couple_lhs :
-  ∀ ℓ v ℓ₀ ℓ₁ h,
-    ℓ₀ != ℓ →
-    ℓ₁ != ℓ →
+  ∀ (ℓ : Location) v (ℓ₀ ℓ₁ : Location) h,
+    ℓ₀.1 != ℓ.1 →
+    ℓ₁.1 != ℓ.1 →
     put_pre_cond ℓ v (couple_lhs ℓ₀ ℓ₁ h).
 Proof.
   intros ℓ v ℓ₀ ℓ₁ h n₀ n₁ s₀ s₁ hc.
@@ -560,9 +575,9 @@ Qed.
   : ssprove_invariant.
 
 Lemma put_pre_cond_couple_rhs :
-  ∀ ℓ v ℓ₀ ℓ₁ h,
-    ℓ₀ != ℓ →
-    ℓ₁ != ℓ →
+  ∀ (ℓ : Location) v (ℓ₀ ℓ₁ : Location) h,
+    ℓ₀.1 != ℓ.1 →
+    ℓ₁.1 != ℓ.1 →
     put_pre_cond ℓ v (couple_rhs ℓ₀ ℓ₁ h).
 Proof.
   intros ℓ v ℓ₀ ℓ₁ h n₀ n₁ s₀ s₁ hc.
@@ -575,10 +590,10 @@ Qed.
   : ssprove_invariant.
 
 Lemma put_pre_cond_triple_rhs :
-  ∀ ℓ v ℓ₁ ℓ₂ ℓ₃ h,
-    ℓ₁ != ℓ →
-    ℓ₂ != ℓ →
-    ℓ₃ != ℓ →
+  ∀ (ℓ : Location) v (ℓ₁ ℓ₂ ℓ₃ : Location) h,
+    ℓ₁.1 != ℓ.1 →
+    ℓ₂.1 != ℓ.1 →
+    ℓ₃.1 != ℓ.1 →
     put_pre_cond ℓ v (triple_rhs ℓ₁ ℓ₂ ℓ₃ h).
 Proof.
   intros ℓ v ℓ₁ ℓ₂ ℓ₃ h n₁ n₂ n₃ s₀ s₁ hc.
@@ -949,7 +964,7 @@ Qed.
 
 Lemma put_pre_cond_rem_lhs :
   ∀ ℓ v ℓ' v',
-    ℓ' != ℓ →
+    ℓ'.1 != ℓ.1 →
     put_pre_cond ℓ v (rem_lhs ℓ' v').
 Proof.
   intros ℓ v ℓ' v' hn s₀ s₁ hc.
@@ -963,7 +978,7 @@ Qed.
 
 Lemma put_pre_cond_rem_rhs :
   ∀ ℓ v ℓ' v',
-    ℓ' != ℓ →
+    ℓ'.1 != ℓ.1 →
     put_pre_cond ℓ v (rem_rhs ℓ' v').
 Proof.
   intros ℓ v ℓ' v' hn s₀ s₁ hc.
@@ -1026,6 +1041,7 @@ Inductive heap_val :=
 Definition loc_val_pair (ℓ : Location) (v : ℓ) : ∑ ℓ : Location, ℓ :=
   (ℓ ; v).
 
+(*
 Definition heap_val_eq : rel heap_val :=
   λ u v,
     match u, v with
@@ -1049,6 +1065,7 @@ Qed.
 HB.instance Definition _ := hasDecEq.Build heap_val heap_val_eqP.
 
 Derive NoConfusion for heap_val.
+ *)
 
 Fixpoint update_pre (l : list heap_val) (pre : precond) :=
   match l with
@@ -1175,6 +1192,7 @@ Proof.
     split. all: split. all: auto.
 Qed.
 
+(*
 Definition cast_loc_val {ℓ ℓ' : Location} (e : ℓ = ℓ') (v : ℓ) : ℓ'.
 Proof.
   subst. auto.
@@ -1189,7 +1207,9 @@ Proof.
   { apply eq_irrelevance. }
   subst. reflexivity.
 Qed.
+ *)
 
+(*
 Equations? lookup_hpv_l (ℓ : Location) (l : seq heap_val) : option ℓ :=
   lookup_hpv_l ℓ (hpv_l ℓ' v' :: l) with inspect (ℓ == ℓ') := {
   | @exist true e => Some (cast_loc_val _ v')
@@ -1375,6 +1395,7 @@ Proof.
   - eapply lookup_hpv_l_None_spec. all: eauto.
   - eapply lookup_hpv_r_None_spec. all: eauto.
 Qed.
+*)
 
 (** Predicate of preservation of precond after updates, retaining memory *)
 
@@ -1470,13 +1491,16 @@ Proof.
   intros s₀ s₁ hh.
   simpl. destruct update_heaps eqn:e.
   intros ℓ₀ hℓ₀.
-  destruct (ℓ₀ != ℓ) eqn:e1.
+  destruct (ℓ₀.1 != ℓ.1) eqn:e1.
   - rewrite !get_set_heap_neq. 2,3: auto.
     eapply h in hh. rewrite e in hh.
     apply hh. auto.
   - move: e1 => /eqP e1. subst.
+  Admitted.
+  (*
     rewrite !get_set_heap_eq. reflexivity.
 Qed.
+   *)
 
 #[export] Hint Extern 10 (preserve_update_mem _ _ (heap_ignore _)) =>
   eapply preserve_update_cons_sym_heap_ignore
@@ -1492,15 +1516,18 @@ Proof.
   intros s₀ s₁ hh.
   simpl. destruct update_heaps eqn:e.
   intros ℓ₀ hℓ₀.
-  destruct (ℓ₀ != ℓ) eqn:e1.
+  destruct (ℓ₀.1 != ℓ.1) eqn:e1.
   - rewrite get_set_heap_neq. 2: auto.
     eapply h in hh. rewrite e in hh.
     apply hh. auto.
   - move: e1 => /eqP e1. subst.
     destruct ℓ.
     move: hℓ₀ => /dommPn //= H.
+Admitted.
+(*
     rewrite hin // in H.
 Qed.
+ *)
 
 #[export] Hint Extern 10 (preserve_update_mem _ _ (heap_ignore _)) =>
   eapply preserve_update_l_ignored_heap_ignore ; [
@@ -1519,15 +1546,18 @@ Proof.
   intros s₀ s₁ hh.
   simpl. destruct update_heaps eqn:e.
   intros ℓ₀ hℓ₀.
-  destruct (ℓ₀ != ℓ) eqn:e1.
+  destruct (ℓ₀.1 != ℓ.1) eqn:e1.
   - rewrite get_set_heap_neq. 2: auto.
     eapply h in hh. rewrite e in hh.
     apply hh. auto.
   - move: e1 => /eqP e1. subst.
     destruct ℓ.
     move: hℓ₀  => /dommPn //= H.
+Admitted.
+(*
     rewrite hin // in H.
 Qed.
+ *)
 
 #[export] Hint Extern 10 (preserve_update_mem _ _ (heap_ignore _)) =>
   eapply preserve_update_r_ignored_heap_ignore ; [
@@ -1593,6 +1623,7 @@ Qed.
   progress (eapply preserve_update_filter_triple_rhs ; simpl)
 : ssprove_invariant.
 
+(*
 Lemma preserve_update_couple_lhs_lookup :
   ∀ ℓ ℓ' (R : _ → _ → Prop) v v' (l : seq heap_val) m,
     lookup_hpv_l ℓ l = Some v →
@@ -1721,6 +1752,7 @@ Proof.
   eapply remember_pre_pre in hh.
   auto.
 Qed.
+ *)
 
 (*
 Lemma preserve_update_loc_rel_lookup_None :
